CleanQ/CleanQ_RBModel.thy
@@ -261,7 +261,6 @@ definition CleanQ_RB_enq_x :: "'a \<Rightarrow> 'a CleanQ_RB_State  \<Rightarrow
 definition CleanQ_RB_enq_y :: "'a \<Rightarrow> 'a CleanQ_RB_State  \<Rightarrow> 'a CleanQ_RB_State"
   where "CleanQ_RB_enq_y b rb = rb \<lparr> rSY := (rSY rb) - {b}, rTYX := rb_enq b (rTYX rb) \<rparr>"
 
-
 text \<open>
   The enqueue operation cannot proceed if there is no space in the corresponding ring
   buffer.
@@ -887,6 +886,40 @@ lemma CleanQ_RB_deq_y_all_inv :
   using can_deq invariants CleanQ_RB_deq_y_I4 CleanQ_RB_deq_y_I3 CleanQ_RB_deq_y_I2 CleanQ_RB_deq_y_I1
   unfolding CleanQ_RB_deq_y_def
   by (metis CleanQ_RB_Invariants.elims(3))
+
+(* ==================================================================================== *)
+subsection \<open>Integration in SIMPL\<close>
+(* ==================================================================================== *)
+
+lemma CleanQ_RB_enq_x_preserves_invariants : 
+  "\<Gamma>\<turnstile> \<lbrace> rb' = \<acute>RingRB \<and> CleanQ_RB_Invariants K \<acute>RingRB \<and> b \<in> rSX \<acute>RingRB \<and> 
+        CleanQ_RB_enq_x_possible \<acute>RingRB \<rbrace> 
+        \<acute>RingRB :== (CleanQ_RB_enq_x b \<acute>RingRB) 
+      \<lbrace> CleanQ_RB_Invariants K \<acute>RingRB \<rbrace>" 
+  apply(vcg)
+  by (meson CleanQ_RB_enq_x_inv_all) 
+
+lemma CleanQ_RB_enq_y_preserves_invariants : 
+  "\<Gamma>\<turnstile> \<lbrace> rb' = \<acute>RingRB \<and> CleanQ_RB_Invariants K \<acute>RingRB \<and> b \<in> rSY \<acute>RingRB \<and> 
+        CleanQ_RB_enq_y_possible \<acute>RingRB \<rbrace> 
+        \<acute>RingRB :== (CleanQ_RB_enq_y b \<acute>RingRB) 
+      \<lbrace> CleanQ_RB_Invariants K \<acute>RingRB \<rbrace>" 
+  apply(vcg)
+  by (meson CleanQ_RB_enq_y_inv_all) 
+
+lemma CleanQ_RB_deq_x_preserves_invariants : 
+  "\<Gamma>\<turnstile> \<lbrace> rb' = \<acute>RingRB \<and> CleanQ_RB_Invariants K \<acute>RingRB \<and> CleanQ_RB_deq_x_possible \<acute>RingRB \<rbrace> 
+        \<acute>RingRB :== (CleanQ_RB_deq_x \<acute>RingRB) 
+      \<lbrace> CleanQ_RB_Invariants K \<acute>RingRB \<rbrace>" 
+  apply(vcg)
+  using CleanQ_RB_deq_x_all_inv by blast
+  
+lemma CleanQ_RB_deq_y_preserves_invariants : 
+  "\<Gamma>\<turnstile> \<lbrace> rb' = \<acute>RingRB \<and> CleanQ_RB_Invariants K \<acute>RingRB \<and> CleanQ_RB_deq_y_possible \<acute>RingRB \<rbrace> 
+        \<acute>RingRB :== (CleanQ_RB_deq_y \<acute>RingRB) 
+      \<lbrace> CleanQ_RB_Invariants K \<acute>RingRB \<rbrace>" 
+  apply(vcg)
+  using CleanQ_RB_deq_y_all_inv by blast
 
 (* ==================================================================================== *)
 subsection \<open>Pre- and post- conditions\<close>
